aarch64 aspec+ainvs: symbolic vs_index_len
Making vs_index_len a sybmolic value instead of a plain number means we
have to unfold config_ARM_PA_SIZE_BITS_40 less often (instead, we need
to consider both cases, which forces us to stay generic).

This also makes sure the type vs_index_len is always distinct from
pt_index_len (even if the sizes are the same), which was only
guaranteed in one of the two configurations before.

Signed-off-by: Gerwin Klein <gerwin.klein@proofcraft.systems>

spec/abstract/AARCH64/Arch_Structs_A.thy
@@ -76,22 +76,51 @@ datatype pte =
       (pte_base_addr : paddr)
 
 
-(* A dependent-ish type in Isabelle: *)
-value_type vs_index_len = "if config_ARM_PA_SIZE_BITS_40 then 10 else (9::nat)"
-type_synonym vs_index = "vs_index_len word"
+definition vs_index_bits :: nat where
+  "vs_index_bits \<equiv> if config_ARM_PA_SIZE_BITS_40 then 10 else (9::nat)"
 
-(* Use vs_index_len instead of vs_index_len_def in generic proofs *)
-lemma vs_index_len:
-  "vs_index_len = (if config_ARM_PA_SIZE_BITS_40 then 10 else (9::nat))"
-  by (simp add: vs_index_len_def Kernel_Config.config_ARM_PA_SIZE_BITS_40_def)
+lemma vs_index_bits_ge0[simp, intro!]: "0 < vs_index_bits"
+  by (simp add: vs_index_bits_def)
+
+(* A dependent-ish type in Isabelle. We use typedef here instead of value_type so that we can
+   retain a symbolic value (vs_index_bits) for the size of the type instead of getting a plain
+   number such as 9 or 10. *)
+typedef vs_index_len = "{n :: nat. n < vs_index_bits}" by auto
+
+end
+
+instantiation AARCH64_A.vs_index_len :: len0
+begin
+  interpretation Arch .
+  definition len_of_vs_index_len: "len_of (x::vs_index_len itself) \<equiv> CARD(vs_index_len)"
+  instance ..
+end
+
+instantiation AARCH64_A.vs_index_len :: len
+begin
+  interpretation Arch .
+  instance
+  proof
+   show "0 < LENGTH(vs_index_len)"
+     by (simp add: len_of_vs_index_len type_definition.card[OF type_definition_vs_index_len])
+  qed
+end
+
+context Arch begin global_naming AARCH64_A
+
+type_synonym vs_index = "vs_index_len word"
 
 type_synonym pt_index_len = 9
 type_synonym pt_index = "pt_index_len word"
 
 text \<open>Sanity check:\<close>
+lemma length_vs_index_len[simp]:
+  "LENGTH(vs_index_len) = vs_index_bits"
+  by (simp add: len_of_vs_index_len type_definition.card[OF type_definition_vs_index_len])
+
 lemma vs_index_ptTranslationBits:
   "ptTranslationBits True = LENGTH(vs_index_len)"
-  by (simp add: ptTranslationBits_def Kernel_Config.config_ARM_PA_SIZE_BITS_40_def)
+  by (simp add: ptTranslationBits_def vs_index_bits_def)
 
 lemma pt_index_ptTranslationBits:
   "ptTranslationBits False = LENGTH(pt_index_len)"
